function method

examples/iterators/DupElements.dfy
@@ -1,105 +1,7 @@
 include "../../src/linear/layer1/List.dfy"
 include "../../src/linear/layer2/LinkedList.dfy"
 include "../../src/linear/layer2/ArrayList.dfy"
-
-function Dup<A>(xs: seq<A>): seq<A>
-{
-  if xs == [] then
-    []
-  else
-    [xs[0]] + [xs[0]] + Dup(xs[1..])
-}
-
-// This is the map that proves the subsequence property
-function DupMap<A>(xs: seq<A>):map<int,int>
-{
- map i | 0<=i<|xs| :: 2*i
-}
-
-function DupRev<A>(xs: seq<A>): seq<A>
-  ensures 2*|xs| == |DupRev(xs)|
-{
-  if xs == [] then
-    []
-  else
-    DupRev(xs[..|xs|-1]) + [xs[|xs|-1]] + [xs[|xs|-1]]
-}
-
-lemma DupDupRev<A>(xs: seq<A>)
-  ensures Dup(xs) == DupRev(xs)
- {
-   if |xs| <=1 {
-   } else
-    {
-     calc == {
-       Dup(xs);
-       [xs[0]] + [xs[0]] + Dup(xs[1..]);
-       [xs[0]] + [xs[0]] + DupRev(xs[1..]);
-       {assert |xs[1..]|==|xs|-1 >=1;
-       assert xs[1..][|xs|-2]== xs[|xs|-1];
-       assert xs[1..][..|xs|-2]== xs[1..|xs|-1];}
-       [xs[0]] + [xs[0]]  + (DupRev(xs[1..|xs|-1]) + [xs[|xs|-1]] + [xs[|xs|-1]]);
-       DupRev(xs[..|xs|-1]) + [xs[|xs|-1]] + [xs[|xs|-1]];
-       DupRev(xs);
-     }
-   }
- }
-
-lemma {:induction xs} setDup<A>(xs: seq<A>)
-ensures forall x :: x in xs <==> x in Dup(xs)
-ensures |Dup(xs)|==2*|xs|
-ensures forall i | 0<=i<|xs| :: xs[i]==Dup(xs)[2*i]==Dup(xs)[2*i+1]
-{}
-
- lemma {:induction xs} dupElsAux<A>(xs: seq<A>,x:A)
- requires x in xs
- ensures multiset(Dup(xs))[x]==2*multiset(xs)[x]
-{
-    if (xs==[]){}
-    else{
-      if (x==xs[0]){
-          if (xs[0] in xs[1..]){
-            calc=={
-              multiset(Dup(xs))[xs[0]];
-              2+multiset(Dup(xs[1..]))[xs[0]];
-              2+2*multiset(xs[1..])[xs[0]];
-              2*(1+multiset(xs[1..])[xs[0]]);{assert xs==[xs[0]]+xs[1..];}
-              2*multiset(xs)[xs[0]];
-            }
-        }
-        else {
-            assert xs[0] !in xs[1..];
-            calc=={
-              multiset(Dup(xs))[xs[0]];
-              2+multiset(Dup(xs[1..]))[xs[0]];
-              {setDup(xs[1..]);
-              assert xs[0] !in xs[1..] ==> xs[0] !in Dup(xs[1..]);
-              assert multiset(Dup(xs[1..]))[xs[0]]==0;}
-              2;{assert xs==[xs[0]]+xs[1..];
-                assert multiset(xs)[xs[0]]==1;}
-              2*multiset(xs)[xs[0]];
-            }
-      }
-      }
-      else {
-        calc=={
-         multiset(Dup(xs))[x];
-         multiset(Dup(xs[1..]))[x];{assert x in xs[1..];}
-         2*multiset(xs[1..])[x];{assert xs==[xs[0]]+xs[1..];}
-         2*multiset(xs)[x];
-       }
-      }
-    }
-}
-
-lemma {:induction xs} dupEls<A>(xs: seq<A>)
- ensures forall x | x in xs :: multiset(Dup(xs))[x]==2*multiset(xs)[x]
-{ forall x | x in xs
-  ensures multiset(Dup(xs))[x]==2*multiset(xs)[x]{
-   dupElsAux(xs,x);
-  }
-}
-
+include "Dup_Utils.dfy"
 
 method DupElements<A>(l: LinkedList<A>)
   modifies l, l.Repr()
@@ -124,7 +26,7 @@ method DupElements<A>(l: LinkedList<A>)
   var it := l.Begin();
   var b := it.HasNext();
 
-    ghost var i := 0;
+  ghost var i := 0;
 
   while b
     decreases |l.Model()| - it.Index()
