examples/iterators/Dup_Utils.dfy
@@ -1,0 +1,133 @@
+function Dup<A>(xs: seq<A>): seq<A>
+{
+  if xs == [] then
+    []
+  else
+    [xs[0]] + [xs[0]] + Dup(xs[1..])
+}
+
+//This is the map that proves the subsequence property
+function DupMap<A>(xs: seq<A>):map<int,int>
+{
+ map i | 0<=i<|xs| :: 2*i
+}
+
+
+function DupRev<A>(xs: seq<A>): seq<A>
+  ensures 2*|xs| == |DupRev(xs)|
+{
+  if xs == [] then
+    []
+  else
+    DupRev(xs[..|xs|-1]) + [xs[|xs|-1]] + [xs[|xs|-1]]
+}
+
+lemma DupDupRev<A>(xs: seq<A>)
+  ensures Dup(xs) == DupRev(xs)
+ {
+   if |xs| <=1 {
+   } else
+    {
+     calc == {
+       Dup(xs);
+       [xs[0]] + [xs[0]] + Dup(xs[1..]);
+       [xs[0]] + [xs[0]] + DupRev(xs[1..]);
+       {assert |xs[1..]|==|xs|-1 >=1; 
+       assert xs[1..][|xs|-2]== xs[|xs|-1];
+       assert xs[1..][..|xs|-2]== xs[1..|xs|-1];}
+       [xs[0]] + [xs[0]]  + (DupRev(xs[1..|xs|-1]) + [xs[|xs|-1]] + [xs[|xs|-1]]);
+       DupRev(xs[..|xs|-1]) + [xs[|xs|-1]] + [xs[|xs|-1]];
+       DupRev(xs);
+     }
+   }
+ }
+
+
+
+
+lemma {:induction xs} setDup<A>(xs: seq<A>)
+ensures forall x :: x in xs <==> x in Dup(xs)
+ensures |Dup(xs)|==2*|xs|
+ensures forall i | 0<=i<|xs| :: xs[i]==Dup(xs)[2*i]==Dup(xs)[2*i+1]
+{}
+
+ lemma {:induction xs} dupElsAux<A>(xs: seq<A>,x:A)
+ requires x in xs
+ ensures multiset(Dup(xs))[x]==2*multiset(xs)[x]
+{
+    if (xs==[]){}
+    else{
+      if (x==xs[0]){
+          if (xs[0] in xs[1..]){
+            calc=={
+              multiset(Dup(xs))[xs[0]];
+              2+multiset(Dup(xs[1..]))[xs[0]];
+              2+2*multiset(xs[1..])[xs[0]];
+              2*(1+multiset(xs[1..])[xs[0]]);{assert xs==[xs[0]]+xs[1..];}
+              2*multiset(xs)[xs[0]];
+            }
+        }
+        else {
+            assert xs[0] !in xs[1..];
+            calc=={
+              multiset(Dup(xs))[xs[0]];
+              2+multiset(Dup(xs[1..]))[xs[0]];
+              {setDup(xs[1..]);
+              assert xs[0] !in xs[1..] ==> xs[0] !in Dup(xs[1..]);
+              assert multiset(Dup(xs[1..]))[xs[0]]==0;}
+              2;{assert xs==[xs[0]]+xs[1..];
+                assert multiset(xs)[xs[0]]==1;}
+              2*multiset(xs)[xs[0]];
+            }
+      }
+      }
+      else {
+        calc=={
+         multiset(Dup(xs))[x];
+         multiset(Dup(xs[1..]))[x];{assert x in xs[1..];}
+         2*multiset(xs[1..])[x];{assert xs==[xs[0]]+xs[1..];}
+         2*multiset(xs)[x];
+       }
+
+
+      }    
+
+
+    }
+
+}
+
+
+lemma {:induction xs} dupEls<A>(xs: seq<A>)
+ ensures forall x | x in xs :: multiset(Dup(xs))[x]==2*multiset(xs)[x]
+{ forall x | x in xs 
+  ensures multiset(Dup(xs))[x]==2*multiset(xs)[x]{
+   dupElsAux(xs,x);
+
+  }
+}
+
+
+function dup(i:int,j:int):int
+ensures i==j==> dup(i,j)==2*i
+ensures i!=j ==> dup(i,j)==2*i+1
+{if (i==j) then 2*i
+ else 2*i+1}
+ 
+
+function fdup(j:int):(int -> int) 
+{ i => dup(i,j)}
+
+
+function dupInvariant(i:int,j:int):int
+ensures i<j==> dupInvariant(i,j)==2*i+1
+ensures i>=j ==> dupInvariant(i,j)==j+i
+{if (i < j) then 2*i+1
+ else i+j}
+
+
+function fdupInvariant(j:int):(int -> int) 
+{ i => dupInvariant(i,j) }
+
+function dupMap<A>(xs:seq<A>,i:int):map<int,int>
+{map it | 0<=it<=|xs| :: if (it < i) then 2*it+1 else i+it}
